# Number Theoretic Algorithms
## GCD Euclid's Algorithm
  ```c
  function Euclid (a,b)
  Input: Two integers a and b with a >=b >= 0
  output: gcd(a,b)

  if b=0: return a
  return Euclid(b,a mod b)
  ```
  - If x and y are positive integers with x >= y, then gcd(x,y) = gcd(x mod y,y)
  ### Proof
   - It is enough to show that gcd(x,y) = gcd(x-y,y) from which the one stated can be derived by repeatedly substracying y from x
   - Any integer that divides both x and y must also divide x-y, so gcd(x,y) <= gcd(x-y,y).
   - Likewise, any integer that divides both x-y and y must also divide both x and y, so gcd(x,y) >= gcd(x-y,y)
  ### Analysis
   - If a >= b, then a mod b < a/2
   #### Proof
   - Witness that either b <= a/2 or b > a/2
   - if b <=, then we have a mod b < b <= a/2
   - if b > a/2 then a mod b = a-b < a/2
   ![image](https://user-images.githubusercontent.com/71220864/137000667-bf127bb3-a146-4799-8313-3f124a9f6d69.png)<br><br>
   - Euclid algorithm is an optimum algorithm
   - The overall run time will be bounded by 2loga (base 2) which is O(loga)

## Extended Euclid's algorithm
  - If d divides both a and b, and d = ax+by for some integers x and y, then necessarily d = gcd(ax+by)
  ### Proof
   - By the first two conditions, d is a common divisor of a and b so it cannot exceed the greatest common divisor, that is, d <= gcd(a,b)
   - On the other hand, since gcd(a,b) is a common divisor of both a and b, it must also divide ax+by = d , which implies gcd(a,b) <= d.
   - Thus from d <= gcd(a,b) and d >= gcd(a,b), we get d = gcd(a,b)
  
  ### How to find such x and y
   - Example: to compute gcd(25,11), Euclid's algorithm would proceed as follows:<br><br>
   ![image](https://user-images.githubusercontent.com/71220864/137001844-a1caad6b-38f9-4ce3-92bd-b95e3a001f4d.png)<br><br>
   ```c
   function extended-Euclid(a,b)
   Input: two positive integers a and b with a >= b >= 0
   Output: Integers x,y,d such that d = gcd(a,b) and ax+by = d
   
   if b = 0: return(1,0,a)
   (x',y',d) = extended-Euclid(b,a mod b)
   return (y',x'- ay'/b,d)
   ```
   - Lemma: For any positive integers a and b, the extended Euclid algorithm returns integers x.y and d such that gcd(a,b) = d = ax+by
   - Inductive Hypothesis: gcd(b,a mod b) = bx' + (a mod b)y'
   - Writing (a mod b) as (a - (a/b)b) we find:<br>
   ![equation](https://latex.codecogs.com/png.latex?%5Cbg_white%20d%20%3D%20gcd%28a%2Cb%29%3D%20gcd%28b%2Ca%5C%20mod%5C%20b%29%20%3D%20bx%27&plus;%28a%20%5C%20mod%5C%20b%29y%27%20%3D%20bx%27%20&plus;%20%28a-%5Cfrac%7Ba%7D%7Bb%7Db%29y%27%3D%20ay%27%20&plus;%20b%28x%27-%5Cfrac%7Ba%7D%7Bb%7Dy%27%29)<br>

## Modular Division
  - We say x is the multiplicative inverse of a modulo N if ax is congruent to 1 (mod N)
  ### Modular division theorem
   - For any a mod N, a has a multiplicative inverse modulo N if and only if it is relatively prime to N. When this inverse exists, it can be found in time O(n³) (where as usual n denotes the number of bits of N) by running the extended Euclid algorithm.
   - Example. Continuing with our previous example, suppose we wish to compute 11- mod 25.
   - Using the extended Euclid algorithm, we find that 15 - 25 – 34 -11 = 1. Reducing both sides modulo 25, we have –34 - 11 = 1 mod 25. So –34 = 16 mod 25 is the inverse of 11 mod 25.
   
## Public key cryptography
  ### How to *Publish* the key and yet be *Secure*?
   #### Ease/Speed of Operation Depends on The Representation
   - viii * xvi = cXxviii
   - 8 * 16 = 128
   - 2^3 * 2^4 = 2^7

   - viii + xvi = xxiv
   - 8 + 16 = 24
   - 2^3 + 2^4 = 2^3.3

   - viii < ix is true
   - 8 < 9 is true
   -  2^3 < 3^2 is true
  
   - Thus if we represent the numbers appropriately, we can perform a particular operation very fast and easily<br><br>
   ![image](https://user-images.githubusercontent.com/71220864/137005082-45ea27e5-033d-44e6-86f9-0320d02247a0.png)<br><br>
  
  ### Using variable speed of operations in cryptography
   - We use this slowness in public key cryptography<br><br>
   ![image](https://user-images.githubusercontent.com/71220864/137005732-1e8fa8ec-5309-493f-a976-ca54faa3683b.png)<br><br>
   - In the above diagram: In representation R2:
    - Operation Ek will be fast 
    - Operation Ek^-1 will be very slow
   - In representation R1
    - Operation Ek^-1 is fast
  ### Example RSA Cryptosystem
  - R1: Product of primes
  - R2: Decimal
  - Ek: Modular Exponentiation m^e mod k

## RSA
  - Pick any two primes p and q and let N = pq.
  - For any e relatively prime to (p -1)(q - 1):
   - The mapping f(x) = x^e mod N is a bijection on {0, 1, ... N-1}
   - Moreover, the inverse mapping is easily realized:
  - let d be the inverse of e modulo (p -1)(q - 1).
  - Then for all x in {0,...N-1}
  - (x^e)^d mod N = x mod N
  ### Correctness
   ![equation](https://latex.codecogs.com/png.latex?%5Cbg_white%20x%5E%7Bed%7D-x%3Dx%5E%7B1&plus;k%28p-1%29%28q-1%29%7D-x)<br>
   - The above is always 0 modulo N. The second form of the expression is convenient because it can be simplified using Fermat's little theorem. It is divible by p(since x^(p-1) = 1 mod p)and likewise by q. Since pand q are primes, this expression must also be divisible by their product N. Hence x^ed - x = x^(1+k(p-1)(q-1)) - x = 0 (mod N), exactly as we need.  
 
## Fermat's little theorem
  - If p is prime, then for every 1 <= a < p, a^(p-1) = 1 mod p
  - The number a.i mod p are distinct because if a.i = a.j (mod p) then dividing both sides by a gives i = j mod p. They are non-zero because a.i = 0 similarly implies i = 0. We assume a is non zero and relatively prime to p.
  - {1,2,….p – 1} = {a · 1 mod p, a - 2 mod p, .…, a· (p – 1) mod p}
  - (p-1)! = a^(p-1).(p-1)! (mod p)
  


